

Evaluar  $f(2)$  usando la interpolación lineal, cuadrática y cúbica

X	f(X)
1	0
4	1.386294
5	1.609438
6	1.791752

Lineal

$$F(x) = \frac{f(x_1) - f(x_0)}{x_1 - x_0} (x - x_0) + f(x_0)$$

$$F(2) = \frac{1.386294 - 0}{4 - 1} (2 - 1) + 0 = 0.462098$$

Cuadrática

$$F_2(x) = b_0 + b_1(x - x_0) + b_2(x - x_0)(x - x_1)$$

$$b_0 = f(x_0) = 0$$

$$b_1 = \frac{f(x_1) - f(x_0)}{x_1 - x_0} = \frac{1.386294 - 0}{4 - 1} = 0.462098$$

$$b_2 = \frac{\frac{f(x_2) - f(x_1)}{x_2 - x_1} - \frac{f(x_1) - f(x_0)}{x_1 - x_0}}{x_2 - x_0} = \frac{\frac{1.609438 - 1.386294}{5 - 4} - \frac{1.386294 - 0}{4 - 1}}{5 - 1} = -0.0547385$$

$$F_2(x) = 0 + 0.462098(2 - 1) + (-0.0547385)(2 - 1)(2 - 4)$$

$$F_2(2) = 0.462098 + 0.119477 = 0.581575$$

Cúbica

$$F(x) = f(x_0) + (x-x_0)f(x_1, x_0) + (x-x_0)(x-x_1)f(x_2, x_1, x_0) + (x-x_0)(x-x_1)(x-x_2)f(x_3, x_2, x_1, x_0)$$

$$f(x_3, x_2, x_1, x_0) = \frac{f(x_3, x_2, x_1) - f(x_3, x_2, x_0)}{x_1 - x_0} = \frac{\frac{f(x_3, x_2) - f(x_3, x_1)}{x_2 - x_1} - \frac{f(x_3, x_2) - f(x_3, x_0)}{x_2 - x_0}}{x_3 - x_0}$$

$$b = \frac{\frac{f(x_3) - f(x_2)}{x_3 - x_2} - \frac{f(x_2) - f(x_1)}{x_2 - x_1} - \frac{f(x_3) - f(x_2)}{x_3 - x_2} - \frac{f(x_2) - f(x_0)}{x_2 - x_0}}{x_3 - x_0}$$

$$b_2 = 0.047792$$

$$F(x) = 0.628767$$